theories/ideas/SpineNormalForm.v
@@ -11,9 +11,33 @@ Structure Normalizer :=
     normalizer : forall v : norm_type, M m:{ v' : norm_type & v' =m= v }
   }.
 
+
+Fixpoint nu_args {T} {n : MTele} : (ArgsOf n -> M T) -> M T :=
+  match n as n return (ArgsOf n -> M T) -> M T with
+  | mBase => fun f => \nu a, f a
+  | mTele F => fun f => \nu a, nu_args (n:=F a) (fun args => f (mexistT _ a args))
+  end.
+
+Fixpoint abs_fun_args {n} : forall {P : ArgsOf n -> Type} (args : ArgsOf n), P args -> M (forall args, P args) :=
+  match n as n return
+        forall {P : ArgsOf n -> Type} (args : ArgsOf n), P args -> M (forall args, P args)
+  with
+  | mBase =>
+    fun P a (p : P a) =>
+      M.abs_fun (P:=fun a => P a) a p
+  | mTele F =>
+    fun P '(mexistT _ a args) p =>
+      p <- abs_fun_args (P:=fun args => P (mexistT _ a args)) args p;
+      p <- M.abs_fun (P:=fun a => forall args, P (mexistT _ a args)) a p;
+      M.ret (fun '(mexistT _ a args) => p a args)
+  end
+.
+
+Notation "'\nu_AO' args0 .. args1 ,  t" := (nu_args (fun args0 => .. (nu_args (fun args1 => t)) ..)) (at level 200, args0 binder, args1 binder, t at level 200).
+
 Fixpoint extend_tele {m : MTele} : (ArgsOf m -> MTele) -> MTele :=
   match m as m return (ArgsOf m -> MTele) -> MTele with
-  | mBase => fun n : (unit -> MTele) => n tt
+  | mBase => fun n : (sunit -> MTele) => n stt
   | mTele F =>
     fun n : (ArgsOf (mTele F) -> MTele) =>
       mTele (fun a => extend_tele (fun args => n (mexistT (fun a => ArgsOf (F a)) a args)))
@@ -33,7 +57,7 @@ Fixpoint args_extend {m : MTele} :
                 ArgsOf (n args_m)
               }
     with
-    | mBase => fun n args_n => mexistT _ tt args_n
+    | mBase => fun n args_n => mexistT _ stt args_n
     | mTele F =>
       fun n '(mexistT _ a args) =>
         let '(mexistT _ args_m args_n) := args_extend args in
@@ -42,8 +66,11 @@ Fixpoint args_extend {m : MTele} :
 
 Fixpoint extend_args {m : MTele} : forall {n : ArgsOf m -> MTele},
   forall args_m : ArgsOf m, ArgsOf (n args_m) -> ArgsOf (extend_tele n) :=
-  match m with
-  | mBase => fun _ '(tt) args_n => args_n
+  match m as m return
+        forall {n : ArgsOf m -> MTele},
+        forall args_m : ArgsOf m, ArgsOf (n args_m) -> ArgsOf (extend_tele n)
+  with
+  | mBase => fun _ _ args_n => suTr (f:=fun a => (ArgsOf (_ a))) args_n
   | mTele F => fun _ '(mexistT _ a args_m) args_n => mexistT _ a (extend_args args_m args_n)
   end
 .
@@ -91,7 +118,7 @@ Section SpNF.
     match m as m return
           forall (f : ArgsOf m -> s) (a : ArgsOf m), f a -> apply_sort (curry_sort s f) a
     with
-    | mBase => fun f '(tt) t => t
+    | mBase => fun f _ t => suTr (f:=fun a => S.selem_of (f a)) t
     | mTele F => fun f '(mexistT _ a args) t => curry_sort_apply (m :=F a) t
     end.
 
@@ -109,7 +136,7 @@ Section SpNF.
   Proof.
     revert l H. induction l. intros H.
     - refine p0.
-    - intros. cbn. apply pS. destruct H. cbn. refine (IHl _).
+    - intros. apply pS. destruct H. refine (IHl _).
   Defined.
 
   Definition branches_for_constrs (val : Mutual.Val) n params P :
@@ -122,30 +149,32 @@ Section SpNF.
   Proof.
     intros F.
     refine (@zip_dep_fold_ind (fun x => M x) _ _ _ _ _ _ _). exact (M.ret tt).
-    intros. cbn.
-    refine (M.bind H0 _). intros H1.
-    refine (M.bind (\nu args_c, _ : M (forall args_c, _)) _); cycle 1.
-    intros. refine (M.ret (m: _,_)); cycle 1.
-    exact H1.
-    refine (curry_val (s:=Propₛ) _).
     intros.
-    refine (curry_sort_apply (s:=Propₛ) _). red.
-    apply (X0 a0).
-    refine (M.bind (F _ _ _) _). intros t.
-    refine (M.abs_fun args_c t).
+    refine (M.bind H0 _). intros H1.
+    refine (M.bind (\nu_AO args_c, _) _); cycle 1.
+    - intros.
+      epose (H3 := curry_val (s:=Propₛ) (fun a => curry_sort_apply (s:=Propₛ) (X0 a))).
+      pose (H4 := reduce (RedWhd RedAll) H3).
+      refine (M.ret (m: H4,H1)).
+    (* refine (curry_val (s:=Propₛ) _). *)
+    (* intros. *)
+    (* refine (curry_sort_apply (s:=Propₛ) _). *)
+    (* refine (X0 a0). *)
+    - refine (M.bind (F _ _ _) _). intros t.
+      refine (abs_fun_args args_c t).
   Defined.
 
-  Fixpoint apply_curry_val {s m} : forall {T f a}, @apply_val s m T (curry_val f) a =m= f a :=
-    match m as m return
-         forall {T f a}, @apply_val s m T (curry_val f) a =m= f a
-    with
-    | mBase => fun _ _ 'tt => meq_refl
-    | mTele F =>
-      fun T f '(mexistT _ a args) =>
-        let r := @apply_curry_val s _ (T a) (fun args => f (mexistT _ a args)) args in
-      ltac:(destruct s; refine r)
-    end
-  .
+  (* Fixpoint apply_curry_val {s m} : forall {T f a}, @apply_val s m T (curry_val f) a =m= f a := *)
+  (*   match m as m return *)
+  (*        forall {T f a}, @apply_val s m T (curry_val f) a =m= f a *)
+  (*   with *)
+  (*   | mBase => fun _ _ _ => meq_refl *)
+  (*   | mTele F => *)
+  (*     fun T f '(mexistT _ a args) => *)
+  (*       let r := @apply_curry_val s _ (T a) (fun args => f (mexistT _ a args)) args in *)
+  (*     ltac:(destruct s; refine r) *)
+  (*   end *)
+  (* . *)
 
   Tactic Notation "diff" uconstr(B) uconstr(T) :=
     let rec diff :=
@@ -163,6 +192,9 @@ Section SpNF.
     let T := type of t in
     diff B T.
 
+  (* Arguments M.bind _ _ & _ _. *)
+  Arguments M.abs_fun _ _ _ & _.
+
   Time Definition body_for (val : Mutual.Val) (n : nat)
              (Fix : forall n, MTele_val (MTele_C Typeₛ Propₛ M (SpNFType val n)))
     :
@@ -173,11 +205,11 @@ Section SpNF.
           (fun args_indices : ArgsOf (apply_constT (Inductive.arity _) args_param) =>
              curry_sort_apply
                (s:=Typeₛ)
-               (fun i => M m:{ i' & i' =m= i})
+               (fun i : Inductive.Inhab _ _ => M m:{ i' & i' =m= i})
           )
     in
 
-    branches <- (\nu args_param,
+    branches <- (\nu_AO args_param,
         branches_for_constrs
           val
           n
@@ -191,19 +223,30 @@ Section SpNF.
              let inhab := apply_curry_sort (s:=Typeₛ) inhab in
              let inhab := apply_val (s:=_) inhab args_c in
              let inhab := apply_curry_sort inhab in
-             let arg_i : ArgsOf (mTele (fun i : Inductive.Inhab _ indices => mBase)) :=
-                 mexistT _ inhab (tt : ArgsOf mBase) in
+             let inhab := reduce (RedWhd (RedAll)) inhab in
+             let inhab_type := reduce (RedWhd RedAll) (Inductive.Inhab _ indices) in
+             let arg_i : ArgsOf (mTele (fun i : inhab_type => mBase)) :=
+                 mexistT _ inhab (stt) in
               let t := apply_val (s:=Propₛ) (Fix n) (extend_args args_param (extend_args indices arg_i)) in
               let t := apply_curry_sort t in
+              let t := reduce (RedWhd (RedAll)) t in
               (* coq does not know that [t] has the right type. The problem is
               that [mfix] expresses the type differently from what [Match.Val]
               requires. *)
-              M.coerce t
+              let A := _ in
+              let B := _ in
+              (* let A' := reduce RedVmCompute A in *)
+              (* let B' := reduce RedVmCompute B in *)
+              (* M.print_term A';; *)
+              (* M.print_term B';; *)
+              t <- M.coerce (A:=A) (B:=B) t;
+              M.ret t
+
           )
-          >>= M.abs_fun args_param
+          >>= abs_fun_args args_param
                 );
 
-    t <- (\nu args : ArgsOf (SpNFTele val n),
+    t <- (\nu_AO args : ArgsOf (SpNFTele val n),
                      m <-
                        (let args_param := mprojT1 (args_extend args) in
         let args := mprojT2 (args_extend args) in
@@ -211,26 +254,46 @@ Section SpNF.
         let args := mprojT2 (args_extend args) in
         let arg_i := mprojT1 (args) in
 
-        ltac:(cast' (M (apply_curry_sort (apply_val (pred (mprojT1 _)) (mprojT1 _)) (mprojT1 _))) (M.build_match {|
+        let branches := reduce (RedWhd RedAll) (branches args_param) in
+
+
+        ltac:(cast' (M (apply_curry_sort (apply_val (pred (mprojT1 _)) (mprojT1 _)) (mprojT1 _))) (
+                      M.build_match {|
             Match.mind_entry := nth_of val n;
             Match.param_args := args_param;
             Match.indices := args_indices;
             Match.val := arg_i;
             Match.sort := Propₛ;
             Match.return_predicate := (pred args_param);
-            Match.branches := branches args_param;
+            Match.branches := branches;
           |}))
         );
         (* >>= M.abs_let arg_i _ *)
         (* >>= M.abs_let args_indices _ *)
           (* >>= M.abs_let args_param _ *)
         let m := apply_curry_sort_inv (s:=Propₛ) m in
-        M.abs_fun args m
+        let m := reduce (RedWhd RedAll) m in
+        abs_fun_args args m
          );
     (* As above, we need to convince Coq that we can massage the types. *)
     t <- M.coerce t;
-    M.ret (curry_val (s:=Propₛ) t)
+    let t := reduce (RedWhd RedAll) (curry_val (s:=Propₛ) t) in
+    M.ret (t)
   .
+
+  (* Definition nat_ind := ltac:(mrun (M.inspect_mind nat >>= fun '{|Mutual.val := val|} => M.ret val)). *)
+
+  (* Definition build_match (P : nat -> Prop) (p0: M (P 0)) (pS : forall n, M (P (S n))) (n : nat) : M (P n) := *)
+  (*   M.build_match *)
+  (*     {| *)
+  (*       Match.mind_entry := nth_of nat_ind 0; *)
+  (*       Match.param_args := mBase; *)
+  (*       Match.indices := mBase; *)
+  (*       Match.val := n; *)
+  (*       Match.sort := Propₛ; *)
+  (*       Match.return_predice := P; *)
+  (*       Match.branches :=  *)
+  (*     |}. *)
 
   Fixpoint val_to_sortP m :
     forall T, @MTele_val Propₛ m T -> @MTele_sort Propₛ m T :=
@@ -241,7 +304,7 @@ Section SpNF.
     | mTele F => fun T t x => val_to_sortP (F x) (T x) (t x)
   end.
 
-  Definition build_normalizer_for (val : Mutual.Val) :=
+  Definition build_normalizer_for (val : Mutual.Val):=
     let tele := mTele (fun n => SpNFTele val n) in
     (* we are constructing a fixpoint of the following form:
        mfix F k P_k_1 .. P_k_pk I_k_1 .. I_k_ik (i : T_k P_k_1 .. P_k_pk I_k_1 .. I_k_ik) : M (m:{ i' : i' =m= i }) :=
@@ -252,22 +315,45 @@ Section SpNF.
        | S _ => <normalize and return value of last inductive> (* this is also the default branch *)
        end
      *)
+    (* branches <- *)
+    (*   (\nu k, \nu F, *)
+    (*    t <- body_for val k F; *)
+    (*    t <- M.abs_fun F t; *)
+    (*    M.abs_fun k t *)
+    (*   ); *)
+    let num_inds := NEList.length (Mutual.ind_defs (Mutual.def val)) in
+    let num_inds := reduce RedVmCompute num_inds in
+    (* below [i] will range from [0] to [num_inds - 1]. *)
     branches <-
-      (\nu k, \nu F,
-       t <- body_for val k F;
-       t <- M.abs_fun F t;
-       M.abs_fun k t
-      );
+      (
+        mfix go (i : _) :
+          M (forall k, MTele_val (MTele_C Typeₛ Propₛ M _) -> MTele_val (MTele_C Typeₛ Propₛ M (SpNFType val (i+k)))) :=
+          match Peano_dec.dec_eq_nat (S i) (num_inds) with
+          | or_introl eq =>
+          (* It is rather tedious to prove that
+             [SpNFType val (num_inds - 1 + k) = SpNFType val (num_inds - 1)]
+             so we'll assert this dynamically
+           *)
+            \nu F,
+              let i := reduce RedVmCompute (num_inds - 1) in
+              t <- (body_for val i F);
+              t <- M.abs_fun F t;
+              M.coerce (fun k : nat => t)
+          | or_intror _ =>
+            M.failwith "unimplemented"
+          end
+      ) (0);
     let mfix_ :=
         MFixDef.mfix'
           (m := tele)
           (fun n => SpNFType val n)
           (fun F k => branches k F
           ) in
+   let t := reduce (RedWhd RedAll) (val_to_sortP _ _ (mfix_)) in
     M.ret (mexistT
             (fun val => forall n, MTele_sort (MTele_C Typeₛ Propₛ M (SpNFType val n)))
             val
-            (val_to_sortP _ _ (mfix_))
+            (t)
           )
   .
 
@@ -281,7 +367,7 @@ Section SpNF.
 
 End SpNF.
 
-Set Printing All.
+(* Set Printing All. *)
 Mtac Do (M.inspect_mind nat >>= fun '{|Mutual.val := val|} => M.print_term val).
 
 Let nat_val :=
@@ -296,14 +382,102 @@ Let nat_val :=
       (fun nat : Set =>
        @mcons (@Constructor.Par.Def mBase mBase)
          (Constructor.Par.Build_Def mBase mBase
-            (String (Ascii.Ascii true true true true false false true false) EmptyString) mBase tt)
+            (String (Ascii.Ascii true true true true false false true false) EmptyString) mBase stt)
          (@mcons (@Constructor.Par.Def mBase mBase)
             (Constructor.Par.Build_Def mBase mBase
                (String (Ascii.Ascii true true false false true false true false) EmptyString)
-               (@mTele nat (fun _ : nat => mBase)) (fun _ : nat => tt)) (@mnil (@Constructor.Par.Def mBase mBase)))))
+               (@mTele nat (fun _ : nat => mBase)) (fun _ : nat => stt)) (@mnil (@Constructor.Par.Def mBase mBase)))))
    nat (@mpair nat (mprod (forall _ : nat, nat) unit) O (@mpair (forall _ : nat, nat) unit S tt))).
 
 
 Let x := Eval hnf in build_normalizer_for nat_val.
 
-Timeout 30 Mtac Do (build_normalizer_for nat_val >>= M.print_term).
+Mtac Do Set_Debug_Exceptions.
+Set Unicoq Debug.
+(* Set Printing All. *)
+(* Set Printing Implicit. *)
+
+Ltac what_the_stuck t :=
+  (* idtac t; *)
+  lazymatch t with
+  (* reduction is blocked because of a fixpoint argument that doesn't reduce *)
+  | (fix f x1 {struct x1} := _) ?a1 => what_the_stuck a1
+  | (fix f x1 x2 {struct x1} := _) ?a1 ?a2 => what_the_stuck a1
+  | (fix f x1 x2 {struct x2} := _) ?a1 ?a2 => what_the_stuck a2
+  (* ... *)
+  | ?f ?g =>
+      (* reduction is blocked because of [f] *)
+      what_the_stuck f
+  | match ?v with | _ => _ end =>
+    (* reduction is blocked because of [v] *)
+    what_the_stuck v
+  | _ =>
+    (* reduction is blocked because of [t] itself *)
+    idtac t
+  end.
+
+Axiom k : nat.
+
+Check ltac:(
+  let t := eval cbv in (k + 0) in
+  what_the_stuck t).
+
+
+Let t := Eval cbv in
+(* (MTele_val (MTele_C Typeₛ Propₛ M (SpNFType nat_val (0 + k)))). *)
+(NEList.netuple_nth (0 + k) (Mutual.inds nat_val)).
+Let s : unit := ltac:(let t := eval unfold t in t in what_the_stuck t; refine tt).
+Print s.
+
+Mtac Do (build_normalizer_for
+           nat_val >>=
+           fun '(mexistT _ _ x) =>
+           M.print_term x;;
+           let y := reduce (RedStrong RedAll) (x 0) in
+           M.print_term y;;
+           M.declare dok_Definition "my_great_metaprogram" false y;;
+           M.ret tt).
+
+Set Printing Universes.
+Set Printing All.
+
+Monomorphic Definition false_test :=
+       '{|Mutual.val := val|} <- M.inspect_mind (@False);
+       M.print_term val;;
+       build_normalizer_for
+           val >>=
+           fun '(mexistT _ _ x) =>
+             (* M.print_term x;; *)
+             (* let y := reduce (RedWhd RedAll) (x 0) in *)
+             M.print_term "before_compute";;
+             let y := reduce (RedVmCompute) (x 0) in
+             M.print_term "after_compute";;
+             M.print_term y;;
+             M.print_term "before_declare";;
+             M.declare dok_Definition "my_great_metaprogram_False" false y;;
+             M.print_term "after_declare";;
+             M.ret tt.
+Print false_test.
+Mtac Do false_test.
+
+Mtac Do (
+       '{|Mutual.val := val|} <- M.inspect_mind (@unit);
+       build_normalizer_for
+           val >>=
+           fun '(mexistT _ _ x) =>
+             (* M.print_term x;; *)
+             let y := reduce (RedWhd RedAll) (x 0) in
+             M.print_term y;;
+             M.declare dok_Definition "my_great_metaprogram2" false y;;
+             M.ret tt).
+
+Mtac Do (
+       '{|Mutual.val := val|} <- M.inspect_mind (@list);
+       build_normalizer_for
+           val >>=
+           fun '(mexistT _ _ x) =>
+             (* M.print_term x;; *)
+             let y := reduce (RedWhd RedAll) (x 0) in
+             M.print_term y;;
+             M.declare dok_Definition "my_great_metaprogram2" false y;;
+             M.ret tt).
